\section{Матрицы — Матричные уравнения}

\begin{sagesilent}
    A = matrix(QQ, [[2, 2, -3], [-1, 0, 4], [0, 2, 2]])
    B = matrix(QQ, [[-2, 4, -6], [2, 0, 8], [4, 4, 2]])    
    C = matrix(QQ, [[2, 1, 1], [-1,-1, 4], [1, 0, 3]])
\end{sagesilent}

Дано уравнение:

$-2X\sage{A} - 0.5\sage{B} = \sage{C}$
~\\

Решение уравнения сводится к двум вариантам умножения:
~\\

\begin{minipage}{0.4\textwidth}
	$A*X = B$
	
	$A^{-1}* A*X = A^{-1}*B$
	
	$X = A^{-1}*B$
\end{minipage}
\hfill
\begin{minipage}{0.4\textwidth}
	$X*A=B$
	
	$X*A*A^{-1} = B*A^{-1}$
	
	$X = B*A^{-1}$
	
\end{minipage}

\begin{sagesilent}
	A = -2 * A
	B = -1/2 * B
\end{sagesilent}

~\\

$X * \sage{A} + \sage{B} = \sage{C}$

~\\
\begin{sagesilent}
	K = C - B
	answer = B * A.inverse()
\end{sagesilent}

$X * \sage{A} = \sage{K}$

~\\

$X = \sage{answer}$
